TYPE_descriptor spec; proof until fst loop [skip ci]

src/Lib/DWT/VST/Der_write_tags.v
@@ -42,30 +42,53 @@ Open Scope Z.
 
 Section Der_write_tags.
 
-Fixpoint n_tuple A n := 
-  match n with
-  | O => A
-  | S n => (A * n_tuple A n)%type
-  end.
+Definition type_descr_composites :=
+  ((_name, (tptr tschar)) :: (_xml_tag, (tptr tschar)) ::
+    (_op, (tptr (Tstruct _asn_TYPE_operation_s noattr))) ::
+    (_tags, (tptr tuint)) :: (_tags_count, tuint) ::
+    (_all_tags, (tptr tuint)) :: (_all_tags_count, tuint) ::
+    (_encoding_constraints, (Tstruct _asn_encoding_constraints_s noattr)) ::
+    (_elements, (tptr (Tstruct _asn_TYPE_member_s noattr))) ::
+    (_elements_count, tuint) :: (_specifics, (tptr tvoid)) :: nil).
 
- Eval cbn in  (reptype type_descriptor_s). 
+
+Fixpoint mk_TYPE_descriptor_repr (ls : list (ident * type))  :=
+  match ls with
+    | [] => val
+    | [h] => let (_, t) := h in reptype t
+    | h :: tl => let (_, t) := h in
+                (reptype t * mk_TYPE_descriptor_repr tl)%type
+  end.  
+
+Definition type_descr := mk_TYPE_descriptor_repr type_descr_composites.
+
+Definition get_tags_count (v : type_descr) :=
+  let (_, y) := v in
+  let (_, y) := y in
+  let (_, y) := y in
+  let (_, y) := y in
+  let (x, y) := y in
+        x. 
 
 Definition der_write_tags_spec : ident * funspec :=
   DECLARE _der_write_tags
   WITH td_p : val, td : TYPE_descriptor,
        struct_len: Z, tag_mode : Z, last_tag_form : Z, tag : Z, 
        cb : val, app_key : val,
-       td' : reptype type_descriptor_s
+       td' : type_descr,
+       tags_p : val
   PRE[tptr type_descriptor_s, tuint, tint, tint, tuint, 
       tptr cb_type, tptr tvoid]
-    PROP()
+    PROP(
+      0 <= Zlength (tags td) + 1 <= Int.max_unsigned;
+      get_tags_count td' = Vint (Int.repr (Zlength (tags td)))) 
     PARAMS(td_p; Vint (Int.repr struct_len); Vint (Int.repr tag_mode);
            Vint (Int.repr last_tag_form); Vint (Int.repr tag); cb; app_key)
     GLOBALS()
-    SEP(data_at Tsh type_descriptor_s td'  td_p;
-       func_ptr' dummy_callback_spec cb;
-       data_at_ Tsh enc_key_s app_key;
-       valid_pointer cb)
+    SEP(data_at Tsh type_descriptor_s td' td_p;
+        func_ptr' dummy_callback_spec cb;
+        data_at_ Tsh enc_key_s app_key;
+        valid_pointer cb)
     POST[tint]
     let size := if Val.eq cb nullval then 0 else 32 in
       PROP()
@@ -80,18 +103,51 @@ Definition der_write_tags_spec : ident * funspec :=
           data_at_ Tsh enc_key_s app_key;
           valid_pointer cb).
 
+ Require Import Core.Tactics.
+
 Definition Gprog := ltac:(with_library prog [der_write_tags_spec]).
 
 Theorem bool_der_encode : semax_body Vprog Gprog (normalize_function f_der_write_tags composites)
                                      der_write_tags_spec.
 Proof.
   start_function.
+  unfold get_tags_count in H0.
+  repeat break_let.
   forward.
-  entailer!.
-  admit.
+  rewrite H0.
   forward_if True.
+  *
   forward.
   entailer!.
+  { break_if;
+    unfold der_write_tags;
+    replace (4 <? Zlength (tags td) + 1) with true;
+    auto;
+    symmetry; Zbool_to_Prop; nia. }
+  *
+  forward.
+  entailer!.
+  *
+  forward_if True.
+  **
+  repeat forward.
+  Require Import VstTactics.
+  forward_if ((temp _t'1
+           (Vint (
+                if eq_dec (Int.repr tag_mode) (Int.neg (Int.repr 1))
+                then (if Int.eq (Int.repr (Zlength (tags td))) Int.zero 
+                  then Int.zero else Int.one)
+                else Int.zero))));
+    repeat forward; try rewrite_if_b; try entailer!.
+  forward_if (((temp _t'2
+           (Vint (
+                if eq_dec (Int.repr tag_mode) (Int.neg (Int.repr 1))
+                then (if Int.eq (Int.repr (Zlength (tags td))) Int.zero 
+                  then Int.zero else Int.one)
+                else Int.zero))))); repeat forward; try rewrite_if_b; try entailer!.
+  repeat break_if; try rep_omega.
+  1-3: admit.
+
 Admitted.
 
 End Der_write_tags.
